Start proof of sha3. Definition of game for bad event + game after eager. Some try in the proof

sha3/proof/old/Squeezeless.ec
@@ -1,42 +1,16 @@
+
 (** This is a theory for the Squeezeless sponge: where the ideal
     functionality is a fixed-output-length random oracle whose output
     length is the input block size. We prove its security even when
     padding is not prefix-free. **)
-require import Fun Option Pair Int Real List FSet NewFMap Utils.
-require (*..*) AWord LazyRP LazyRO Indifferentiability.
-(* TODO: Clean up the Bitstring and Word theories
-      -- Make use of those new versions. *)
-(*...*) import Dprod Dexcepted.
-(* TODO: Datatype definitions and distributions should
-     be properly separated and reorganized. *)
+require import Pred Fun Option Pair Int Real List FSet NewFMap Utils Common.
 
-op r : { int | 0 < r } as lt0_r.
-op c : { int | 0 < c } as lt0_c.
+require (*..*) RndOrcl Indifferentiability.
+(*...*) import Dprod Dexcepted Capacity.
 
-(** Clarify assumptions on the distributions as we go. As this is currently
-    written, we are hiding some pretty heavy axioms behind cloning. **)
-type block.
-op dblock: block distr.
+type state  = block  * capacity.
+op   dstate = bdistr * cdistr.
 
-clone import AWord as Block with
-  op   length      <- r,
-  type word        <- block,
-  op   Dword.dword <- dblock
-proof leq0_length by smt.
-
-type capacity.
-op dcapacity: capacity distr.
-
-clone AWord as Capacity with
-  op   length      <- c,
-  type word        <- capacity,
-  op   Dword.dword <- dcapacity
-proof leq0_length by smt.
-
-type state  = block  *  capacity.
-op   dstate = dblock * dcapacity.
-
-print Indifferentiability.
 
 clone include Indifferentiability with
   type p     <- state, 
@@ -45,27 +19,47 @@ clone include Indifferentiability with
   rename [module] "GReal" as "RealIndif"
          [module] "GIdeal"  as "IdealIndif".
 
-(** Ideal Functionality **)
-clone import LazyRO as Functionality with
-  type from <- block list,
-  type to   <- block,
-  op   d    <- dblock.
 
-(** Ideal Primitive for the Random Transformation case **)
-clone import LazyRP as Primitive with
-  type D <- state,
-  op   d <- dstate.
+(* max number of call to the permutation and its inverse *)
+op max_size : int.
+
+(** Ideal Functionality **)
+clone import Tuple as TupleBl with
+  type t <- block,
+  op Support.enum <- Block.words
+  proof Support.enum_spec by exact Block.enum_spec. 
+
+op bl_enum = flatten (mkseq (fun i => wordn i) (max_size + 1)). 
+op bl_univ = FSet.oflist bl_enum.
+
+clone RndOrcl as RndOrclB with 
+  type from <- block list,
+  type to   <- block.
+ 
+clone import RndOrclB.RestrIdeal as Functionality with
+  op sample _ <- bdistr,
+  op test l   <- List.size l <= max_size,
+  op univ     <- bl_univ,
+  op dfl      <- b0
+  proof *.
+realize sample_ll by exact Block.DWord.bdistr_ll.
+realize testP.
+proof.
+  move=> x; rewrite mem_oflist-flattenP; split=>[_|[s[/mkseqP[i[/=_->>]]/wordnP->/#]]].
+  exists (wordn (size x));cut Hsx := size_ge0 x.
+  rewrite wordnP max_ler //= mkseqP /=;exists (size x);smt ml=0.
+qed.
 
 (** We can now define the squeezeless sponge construction **)
 module SqueezelessSponge (P:PRIMITIVE): CONSTRUCTION(P), FUNCTIONALITY = {
   proc init () = {} 
 
   proc f(p : block list): block = {
-    var (sa,sc) <- (Block.zeros,Capacity.zeros);
+    var (sa,sc) <- (b0,c0);
 
-    if (1 <= size p /\ p <> [Block.zeros]) {
+    if (1 <= size p /\ p <> [b0]) {
       while (p <> []) { (* Absorption *)
-        (sa,sc) <@ P.f((sa ^ head witness p,sc));
+        (sa,sc) <@ P.f((sa +^ head witness p,sc));
         p <- behead p;
       }
     }
@@ -73,176 +67,18 @@ module SqueezelessSponge (P:PRIMITIVE): CONSTRUCTION(P), FUNCTIONALITY = {
   }
 }.
 
-(** And the corresponding simulator **)
-op find_chain: (state,state) fmap -> state -> (block list * block) option.
-
-module S (F : FUNCTIONALITY) = {
-  var m, mi: (state,state) fmap
-
-  proc init() = {
-    m  <- map0;
-    mi <- map0;
-  }
-
-  proc f(x:state) = {
-    var pvo, p, v, h, y;
-
-    if (!mem (dom m) x) {
-      pvo <- find_chain m x;
-      if (pvo <> None) {
-        (p,v) <- oget pvo;
-        h <@ F.f(rcons p v);
-        y <$ dcapacity;
-      } else {
-        (h,y) <$ dstate;
-      }
-      m.[x] <- (h,y);
-      mi.[(h,y)] <- x;
-    }
-    return oget m.[x];
-  }
-
-  proc fi(x:state) = {
-    var y;
-
-    if (!mem (dom mi) x) {
-      y <$ dstate;
-      mi.[x] <- y;
-      m.[y] <- x;
-    }
-    return oget mi.[x];
-  }
-}.
-
 section.
-  declare module D : Self.DISTINGUISHER {P, H, S}.
 
-  (** Inlining oracles into the experiment for clarity **)
-  (* TODO: Drop init from the Distinguisher parameters' signatures *)
-  local module Ideal = {
-    var ro : (block list,block) fmap
-    var m, mi : (state,state) fmap
+  declare module D : Self.DISTINGUISHER {Perm, RO}.
 
-    module F = {
-      proc init(): unit = { }
-
-      proc f(x : block list): block = {
-        if (!mem (dom ro) x) {
-          ro.[x] <$ dblock;
-        }
-        return oget ro.[x];
-      }
-    }
-
-    module S = {
-      proc init(): unit = { }
-
-      proc f(x : state): state = {
-        var pvo, p, v, h, y;
-
-        if (!mem (dom m) x) {
-          pvo <- find_chain m x;
-          if (pvo <> None) {
-            (p,v) <- oget pvo;
-            h <@ F.f(rcons p v);
-            y <$ dcapacity;
-          } else {
-            (h,y) <$ dstate;
-          }
-          m.[x] <- (h,y);
-          mi.[(h,y)] <- x;
-        }
-        return oget m.[x];
-      }
-
-      proc fi(x:state) = {
-        var y;
-
-        if (!mem (dom mi) x) {
-          y <$ dstate;
-          mi.[x] <- y;
-          m.[y] <- x;
-        }
-        return oget mi.[x];
-      }
-
-    }
-
-    proc main(): bool = {
-      var b;
-
-      ro <- map0;
-      m  <- map0;
-      mi <- map0;
-      b  <@ D(F,S).distinguish();
-      return b;
-    }
-  }.
-
-  local module Concrete = {
-    var m, mi: (state,state) fmap
-
-    module P = {
-      proc init(): unit = { }
-
-      proc f(x : state): state = {
-        var y;
-
-        if (!mem (dom m) x) {
-          y <$ dstate \ (rng m);
-          m.[x]  <- y;
-          mi.[y] <- x;
-        }
-        return oget m.[x];
-      }
-
-      proc fi(x : state): state = {
-        var y;
-
-        if (!mem (dom mi) x) {
-          y <$ dstate \ (rng mi);
-          mi.[x] <- y;
-          m.[y]  <- x;
-        }
-        return oget mi.[x];
-      }
-
-    }
-
-    module C = {
-      proc init(): unit = { }
-
-      proc f(p : block list): block = {
-        var (sa,sc) <- (Block.zeros,Capacity.zeros);
-
-        if (1 <= size p /\ p <> [Block.zeros]) {
-          while (p <> []) { (* Absorption *)
-            (sa,sc) <@ P.f((sa ^ head witness p,sc));
-            p <- behead p;
-          }
-        }
-        return sa;          (* Squeezing phase (non-iterated) *)
-      }
-    }
-
-    proc main(): bool = {
-      var b;
-
-      m  <- map0;
-      mi <- map0;
-      b  <@ D(C,P).distinguish();
-      return b;
-    }    
-  }.
+  local module Concrete = RealIndif(SqueezelessSponge,Perm,D).
 
   (** Result: The adversary's advantage in distinguishing the modular
       defs is equal to that of distinguishing these **)
   local lemma Inlined_pr &m:
-    `|Pr[RealIndif(SqueezelessSponge,P,D).main() @ &m: res]
-      - Pr[IdealIndif(H,S,D).main() @ &m: res]|
-    = `|Pr[Concrete.main() @ &m: res]
-        - Pr[Ideal.main() @ &m: res]|.
-  proof. by do !congr; expect 2 (byequiv=> //=; proc; inline *; sim; auto). qed.
+     Pr[RealIndif(SqueezelessSponge,Perm,D).main() @ &m: res]
+    = Pr[Concrete.main() @ &m: res].
+  proof. trivial. qed.
 
   (** An intermediate game where we don't care about the permutation
       being a bijection anymore... **)
@@ -280,11 +116,11 @@ section.
       proc init(): unit = { }
 
       proc f(p : block list): block = {
-        var (sa,sc) <- (Block.zeros,Capacity.zeros);
+        var (sa,sc) <- (b0,c0);
 
-        if (1 <= size p /\ p <> [Block.zeros]) {
+        if (1 <= size p /\ p <> [b0]) {
           while (p <> []) { (* Absorption *)
-            (sa,sc) <@ P.f((sa ^ head witness p,sc));
+            (sa,sc) <@ P.f((sa +^ head witness p,sc));
             p <- behead p;
           }
         }
@@ -301,6 +137,13 @@ section.
       return b;
     }
   }.
+  
+  op bound_concrete : real.
+
+  local lemma Concrete_Concrete_F &m: 
+    Pr[Concrete.main() @ &m: res] <=
+    Pr[Concrete_F.main() @ &m: res] + bound_concrete.
+  admitted.
 
   (** Result (expected): The distance between Concrete and Concrete_F
       is bounded by N^2/|state|, where N is the total cost (in terms
@@ -333,7 +176,7 @@ section.
       samplings are independent, hence the move away from a random
       permutation. Some side-effects remain worrying.
    **)
-  type caller = [ | I | D ].
+  type caller = [ I | D ].
 
   op (<=) (o1 o2 : caller) = o1 = I \/ o2 = D.
 
@@ -362,46 +205,521 @@ section.
     by split; apply/half_permutation_set.
   qed.    
 
-print FUNCTIONALITY.
-  local module Game0 = {
-    var m, mi               : (state,state) fmap
-    var mcol, micol         : (state,caller) fmap (* colouring maps for m, mi *)
-    var paths               : (capacity,block list * block) fmap
-    var pathscol            : (capacity,caller) fmap (* colouring maps for paths *)
-    var bext, bred          : bool
-    var bcoll, bsuff, bmitm : bool
+  type handle  = int.
+
+  type hstate = block * handle.
+ 
+  type ccapacity = capacity * caller.
+
+  op hinv (handles:(handle,ccapacity) fmap) (c:capacity) = 
+     find (fun _ => pred1 c \o fst) handles.
+
+  op hinvD (handles:(handle,ccapacity) fmap) (c:capacity) = 
+     find (fun _ => pred1 (c,D)) handles.
+
+  local module G2 = {
+    var m, mi               : (state , state ) fmap
+    var mh, mhi             : (hstate, hstate) fmap
+    var handles             : (handle, ccapacity) fmap
+    var chandle             : int
+    var paths               : (capacity, block list * block) fmap
+    var bext, bcol          : bool
+
+
+    module C = {
+      proc init(): unit = { }
+
+      proc f(p : block list): block = {
+        var h, i <- 0; 
+        var (sa,sc) <- (b0,c0);
+        var sa';
+
+        if (1 <= size p /\ p <> [b0]) {
+          while (i < size p - 1 /\ mem (dom m) (sa +^ nth witness p i, sc)) {
+            (sa, sc) <- oget m.[(sa +^ nth witness p i, sc)];
+            (sa', h) <- oget mh.[(sa +^ nth witness p i, h)];
+            i        <- i + 1;
+          }
+          while (i < size p) {
+            sc                  <$ cdistr;
+            bcol                <- bcol \/ hinv handles sc <> None;
+            sa'                 <- RO.f(take i p);
+            mh.[(sa,h)]         <- (sa', chandle);
+            mhi.[(sa',chandle)] <- (sa,h);
+            (sa,h)              <- (sa',chandle);
+            handles.[chandle]   <- (sc,I);
+            chandle             <- chandle + 1;
+            i                   <- i + 1;
+          }
+          sa <- RO.f(p);
+        }
+        return sa;
+      }
+    }
+
+    module S = {
+      (** Inner interface **)
+      proc f(x : state): state = {
+        var p, v, y, y1, y2, hy2, hx2;
+  
+        if (!mem (dom m) x) {
+          if (mem (dom paths) x.`2) {
+            (p,v) <- oget paths.[x.`2]; 
+            y1    <- RO.f (rcons p (v +^ x.`1));
+            y2    <$ cdistr;
+            y     <- (y1, y2);
+            paths.[y2] <- (rcons p (v +^ x.`1), y.`1);
+          } else {
+            y <$ dstate;
+          }
+          bext <- bext \/ mem (rng handles) (x.`2, I);   
+            (*  exists x2 h, handles.[h] = Some (X2,I) *)
+          if (!(mem (rng handles) (x.`2, D))) {
+            handles.[chandle] <- (x.`2, D);
+            chandle <- chandle + 1;
+          }
+          hx2 <- oget (hinvD handles x.`2);
+          if (mem (dom mh) (x.`1, hx2) /\ (oget handles.[(oget mh.[(x.`1,hx2)]).`2]).`2 = I) {
+            hy2               <- (oget mh.[(x.`1, hx2)]).`2;
+            y                 <- (y.`1, (oget handles.[hy2]).`1);
+            handles.[hy2]     <- (y.`2, D);
+            (* bad               <- bad \/ mem X2 y.`2; *)
+            m.[x]             <- y;
+            mi.[y]            <- x;
+          } else {
+            bcol              <- bcol \/ hinv handles y.`2 <> None;          
+            hy2               <- chandle;
+            chandle           <- chandle + 1;
+            handles.[hy2]     <- (y.`2, D);
+            m.[x]             <- y;
+            mh.[(x.`1, hx2)]  <- (y.`1, hy2);
+            mi.[y]            <- x;
+            mhi.[(y.`1, hy2)] <- (x.`1, hx2);
+          }
+        } else {   
+          y <- oget m.[x];
+        }
+        return y;
+      }
+
+      proc fi(x : state): state = {
+        var y, y1, hx2, hy2;
+
+        if (!mem (dom mi) x) {
+          bext <- bext \/ mem (rng handles) (x.`2, I);   
+            (*  exists x2 h, handles.[h] = Some (X2,I) *)
+          if (!(mem (rng handles) (x.`2, D))) {
+            handles.[chandle] <- (x.`2, D);
+            chandle <- chandle + 1;
+          }
+          hx2 <- oget (hinvD handles x.`2);
+          y                 <$ dstate;
+          if (mem (dom mhi) (x.`1, hx2) /\ (oget handles.[(oget mh.[(x.`1,hx2)]).`2]).`2 = I) {
+            (y1,hy2)          <- oget mhi.[(x.`1, hx2)];
+            y                 <- (y.`1, (oget handles.[hy2]).`1);
+            handles.[hy2]     <- (y.`2, D);
+            (* bad               <- bad \/ mem X2 y.`2; *)
+            mi.[x]            <- y;
+            mhi.[(x.`1, hx2)] <- (y.`1, hy2);
+            m.[y]             <- x;
+            mh.[(y.`1, hy2)]  <- (x.`1, hx2);
+          } else {
+            bcol              <- bcol \/ hinv handles y.`2 <> None;          
+            hy2               <- chandle;
+            chandle           <- chandle + 1;
+            handles.[hy2]     <- (y.`2, D);
+            mi.[x]            <- y;
+            mhi.[(x.`1, hx2)] <- (y.`1, hy2);
+            m.[y]             <- x;
+            mh.[(y.`1, hy2)]  <- (x.`1, hx2);
+          }
+        } else {
+          y <- oget mi.[x];
+        }
+        return y;
+      }
+
+      (** Distinguisher interface **)
+      proc init() = { }
+
+    }
+
+  
+
+    proc main(): bool = {
+      var b;
+
+      m        <- map0;
+      mi       <- map0;
+      bext     <- false;
+      bcol    <- false;
+
+      (* the empty path is initially known by the adversary to lead to capacity 0^c *)
+      handles  <- map0.[0 <- (c0, D)];
+      paths    <- map0.[c0 <- ([<:block>],b0)];
+      chandle  <- 1;
+      b        <@ D(C,S).distinguish();
+      return b;
+    }    
+  }.
+
+op INV2 (m mi:(state , state ) fmap) (mh mhi:(hstate, hstate) fmap) (handles:(handle, ccapacity) fmap) chandle = 
+  dom mh = rng mhi /\ dom mhi = rng mh /\ 
+  (forall xh, mem (dom mh `|` rng mh) xh => mem (dom handles) xh.`2) /\ 
+  (forall h, mem (dom handles) h => h < chandle) /\
+  (forall xh,  mem (dom mh) xh => mem (dom m) (xh.`1, (oget handles.[xh.`2]).`1) \/ (oget handles.[xh.`2]).`2 = I) /\
+  (forall xh,  mem (dom mhi) xh => mem (dom mi) (xh.`1, (oget handles.[xh.`2]).`1) \/ (oget handles.[xh.`2]).`2 = I).
+
+lemma get_oget (m:('a,'b)fmap) (x:'a) : mem (dom m) x => m.[x] = Some (oget m.[x]).
+proof. by rewrite in_dom;case (m.[x]). qed.
+
+lemma find_set (m:('a,'b) fmap) y x (p:'a -> 'b -> bool):
+  (forall x, mem (dom m) x => !p x (oget m.[x])) =>
+  find p m.[x <- y] = if p x y then Some x else None.
+proof.
+  cut [[a []->[]] | []-> Hp Hnp]:= findP p (m.[x<-y]);1: rewrite getP dom_set !inE /#. 
+  by case (p x y)=> //; cut := Hp x;rewrite getP dom_set !inE /= oget_some.
+qed.
+
+require import StdOrder.
+require import Ring.
+
+lemma hinvD_rng x (handles:(handle, ccapacity) fmap):
+   mem (rng handles) (x, D) =>
+                  handles.[oget (hinvD handles x)]= Some(x, D).
+proof.
+  cut[ [a []->[]] | []->/=Hp ]/=:= findP (fun _ z => z = (x, D)) handles.
+  + by rewrite oget_some=> ? <- _;apply get_oget.
+  by rewrite in_rng=> [a Ha];cut := Hp a; rewrite in_dom Ha oget_some. 
+qed.
+
+(* TODO: change the name *)
+lemma map_perm (m mi: ('a, 'a) fmap) x y: !mem (dom mi) y => dom m = rng mi => dom m.[x<-y] = rng mi.[y<- x].
+proof.
+  move=> Hdom Heq;rewrite fsetP=> w;rewrite dom_set in_rng !inE;split.
+  + rewrite Heq in_rng. case (w=x)=>[->|Hneq/=[a Ha]];1:by exists y;rewrite getP. 
+    exists a;rewrite getP;case (a=y)=>[->>|//].
+    by move:Hdom;rewrite in_dom Ha.
+  rewrite Heq in_rng;by move=>[a];rewrite getP;case(a=y)=>[->>/# |_ <-];left;exists a.
+qed.
+
+local hoare test_f : G2.S.f : INV2 G2.m G2.mi G2.mh G2.mhi G2.handles G2.chandle (*/\  INV2 G2.mi G2.mhi G2.handles*) ==>
+                              INV2 G2.m G2.mi G2.mh G2.mhi G2.handles G2.chandle.
+proof.
+  proc;if;last by auto.
+  auto;conseq (_ :_ ==> true)=> //.
+  move=> &hr [][]Hmhmhi[]Hmhimh[]Hdomh[]Hhbound[]Hmhor Hmhior Hnmem y _;split;beta iota.
+  + move=> Hnrng handles chandle hx2 @/handles.
+    cut ->>{hx2} : hx2 = G2.chandle{hr}.  
+    + rewrite /hx2 /handles /hinvD find_set /pred1 //=.
+      move=> x2 Hx2;cut := Hnrng;rewrite in_rng NewLogic.negb_exists /= => /(_ x2).
+      by rewrite get_oget.
+    split=> /= [[Hmem _] | Hmem]. 
+    + by cut /Hhbound // := Hdomh (x{hr}.`1, G2.chandle{hr}) _; rewrite inE;left.
+    do !apply andI. 
+    + apply map_perm=> //;rewrite -not_def=> H.
+      by cut /#:= Hhbound chandle _;apply (Hdomh (y.`1,chandle));rewrite !inE -Hmhimh H.
+    + apply map_perm=> //;rewrite -not_def=> H.
+      by cut /#:= Hhbound G2.chandle{hr} _;apply (Hdomh (x{hr}.`1,G2.chandle{hr}));rewrite !inE H. 
+    + move=>[x1 h];cut := Hdomh (x1,h).
+      rewrite !(dom_set, rng_set, inE) /==>H1 [[H2|[_->]]|[/rng_rem_le H2|[_->]]]//;
+      by rewrite H1 ?H2.
+    + by move=> h;cut := Hhbound h;rewrite !dom_set !inE /= => H [[/H|]|->>]/#.
+    + move=>[x1 h];rewrite !getP !dom_set !inE /==>[|[]->> ->>];rewrite /chandles /=.
+      + move=>Hh. cut /Hhbound/=:= Hdomh (x1,h) _;1:by rewrite !inE Hh.
+        move=> ^Hlt /IntOrder.gtr_eqF; rewrite eq_sym=>->.
+        by cut ->/#: h <> G2.chandle{hr} + 1 by smt ml=0.
+      cut ->/=: G2.chandle{hr} <> G2.chandle{hr} + 1 by smt ml=0.
+      by rewrite oget_some /#. 
+     move=>[x1 h];rewrite !getP !dom_set !inE /==>[|[]->> ->>];rewrite /chandles /=.
+     + move=>Hh; cut /Hhbound/=:= Hdomh (x1,h) _;1:by rewrite !inE -Hmhimh Hh.
+       move=> ^Hlt /IntOrder.gtr_eqF; rewrite eq_sym=>->.
+       by cut ->/#: h <> G2.chandle{hr} + 1 by smt ml=0.
+     by rewrite oget_some /#.
+  move=> /= Hrng;cut Hget:= hinvD_rng _ _ Hrng;split=> /=.
+  + move=> []/Hmhor /= [] ; rewrite Hget oget_some /#.
+  move=> Hnot;do !apply andI. 
+  + apply map_perm=> //;rewrite -not_def=> H.
+    by cut /#:= Hhbound G2.chandle{hr} _;apply (Hdomh (y.`1,G2.chandle{hr}));
+       rewrite !inE -Hmhimh H.
+  + apply map_perm=> //;rewrite -not_def=> H.
+    by cut := Hmhor _ H;move: Hnmem;rewrite Hget oget_some /=;case (x{hr}).
+  + move=> [x1 h];rewrite !(dom_set,rng_set, inE) => [[H|[_ ->]]| [/rng_rem_le H|[_->]]]//=.
+    + by left;apply (Hdomh (x1,h));rewrite inE H.
+    + by left;rewrite in_dom Hget.
+    by left;apply (Hdomh (x1,h));rewrite inE H.
+  + by move=>h;rewrite dom_set !inE=> [/Hhbound|->]/#. 
+  + move=> [x1 h];rewrite !(dom_set, getP, inE) /==>[H|[->> ->>]].
+    + by cut /IntOrder.ltr_eqF->/#:= Hhbound h _;1:by apply (Hdomh (x1,h));rewrite inE H.
+    cut ->/=:oget (hinvD G2.handles{hr} x{hr}.`2) <> G2.chandle{hr}.
+    + by cut /#:= Hhbound (oget (hinvD G2.handles{hr} x{hr}.`2)) _;1:by rewrite in_dom Hget.
+    by rewrite Hget oget_some /=;right;case (x{hr}).
+  move=> [x1 h];rewrite !(dom_set, getP, inE) /==>[H|[->> ->> /=]].
+  + by cut /IntOrder.ltr_eqF->/#:= Hhbound h _;1: apply (Hdomh (x1,h));rewrite inE -Hmhimh H.
+  by rewrite oget_some /=;right;case y.
+qed.
+
+local hoare test_fi : G2.S.fi : INV2 G2.m G2.mi G2.mh G2.mhi G2.handles G2.chandle  ==>
+                                INV2 G2.m G2.mi G2.mh G2.mhi G2.handles G2.chandle.
+proof.
+  proc;if;last by auto.
+  auto.  move=> &hr [][]Hmhmhi[]Hmhimh[]Hdomh[]Hhbound[]Hmhor Hmhior Hnmem;split;beta iota.
+  + move=> Hnrng handles chandle hx2 @/handles y Hy.
+    cut ->>{hx2} : hx2 = G2.chandle{hr}.  
+    + rewrite /hx2 /handles /hinvD find_set /pred1 //=.
+      move=> x2 Hx2;cut := Hnrng;rewrite in_rng NewLogic.negb_exists /= => /(_ x2).
+      by rewrite get_oget.
+    split=> /= [[Hmem _] | Hmem]. 
+    + by cut /Hhbound // := Hdomh (x{hr}.`1, G2.chandle{hr}) _;rewrite inE -Hmhimh;right.
+    do !apply andI. 
+    + apply map_perm=> //;rewrite -not_def=> H.
+      by cut /#:= Hhbound G2.chandle{hr} _;apply (Hdomh (x{hr}.`1,G2.chandle{hr}));
+         rewrite !inE -Hmhimh H.
+    + apply map_perm=> //;rewrite -not_def=> H.
+      by cut /#:= Hhbound chandle _;apply (Hdomh (y.`1,chandle));rewrite !inE -Hmhimh H.
+    + move=>[x1 h];cut := Hdomh (x1,h).
+      rewrite !(dom_set, rng_set, inE) /==>H1 [[H2|[_->]]|[/rng_rem_le H2|[_->]]]//;
+      by rewrite H1 ?H2.
+    + by move=> h;cut := Hhbound h;rewrite !dom_set !inE /= => H [[/H|]|->>]/#.
+    + move=>[x1 h];rewrite !getP !dom_set !inE /==>[|[]->> ->>];rewrite /chandles /=.
+      + move=>Hh; cut /Hhbound/=:= Hdomh (x1,h) _;1:by rewrite !inE -Hmhimh Hh.
+        move=> ^Hlt /IntOrder.gtr_eqF; rewrite eq_sym=>->.
+        by cut ->/#: h <> G2.chandle{hr} + 1 by smt ml=0.
+      by rewrite oget_some /#.
+    move=>[x1 h];rewrite !getP !dom_set !inE /==>[|[]->> ->>];rewrite /chandles /=.
+    + move=>Hh;cut /Hhbound/=:= Hdomh (x1,h) _;1:by rewrite !inE -Hmhimh Hh.
+      move=> ^Hlt /IntOrder.gtr_eqF; rewrite eq_sym=>->.
+      by cut ->/#: h <> G2.chandle{hr} + 1 by smt ml=0.
+    cut ->/=: G2.chandle{hr} <> G2.chandle{hr} + 1 by smt ml=0.
+    by rewrite oget_some /#. 
+  move=> /= Hrng y Hy;cut Hget:= hinvD_rng _ _ Hrng;split=> /=.
+  + move=> []/Hmhior /= [] ; rewrite Hget oget_some /#.
+  move=> Hnot;do !apply andI. 
+  + apply map_perm=> //;rewrite -not_def=> H.
+    by cut := Hmhior _ H;move: Hnmem;rewrite Hget oget_some /=;case (x{hr}).
+  + apply map_perm=> //;rewrite -not_def=> H.
+    by cut /#:= Hhbound G2.chandle{hr} _;apply (Hdomh (y.`1,G2.chandle{hr}));
+       rewrite !inE -Hmhimh H.
+  + move=> [x1 h];rewrite !(dom_set,rng_set, inE) => [[H|[_ ->]]| [/rng_rem_le H|[_->]]]//=.
+    + by left;apply (Hdomh (x1,h));rewrite inE H.
+    + by left;apply (Hdomh (x1,h));rewrite inE H.
+    by left;rewrite in_dom Hget.
+  + by move=>h;rewrite dom_set !inE=> [/Hhbound|->]/#. 
+  + move=> [x1 h];rewrite !(dom_set, getP, inE) /==>[H|[->> ->> /=]].
+    + by cut /IntOrder.ltr_eqF->/#:= Hhbound h _;1: apply (Hdomh (x1,h));rewrite inE -Hmhimh H.
+    by rewrite oget_some /==>{Hy};right;case y.
+  move=> [x1 h];rewrite !(dom_set, getP, inE) /==>[H|[->> ->>]].
+  + by cut /IntOrder.ltr_eqF->/#:= Hhbound h _;1:apply (Hdomh (x1,h));rewrite inE -Hmhimh H.
+  cut ->/=:oget (hinvD G2.handles{hr} x{hr}.`2) <> G2.chandle{hr}.
+  + by cut /#:= Hhbound (oget (hinvD G2.handles{hr} x{hr}.`2)) _;1:by rewrite in_dom Hget.
+  by rewrite Hget oget_some /=;right;case (x{hr}).
+qed.
+
+local hoare test_C : G2.C.f : INV2 G2.m G2.mi G2.mh G2.mhi G2.handles G2.chandle  ==>
+                              INV2 G2.m G2.mi G2.mh G2.mhi G2.handles G2.chandle.
+ 
+
+local module Game3 = {
+    var m, mi               : (state , state ) fmap
+    var mh, mhi             : (hstate, hstate) fmap
+    var handles             : (handle, ccapacity) fmap
+    var chandle             : int
+    var paths               : (capacity, block list * block) fmap
+    var bext                : bool
+
+
+    module C = {
+      proc init(): unit = { }
+
+      proc f(p : block list): block = {
+        var h, i <- 0; 
+        var (sa,sc) <- (b0,c0);
+        var sa';
+
+        if (1 <= size p /\ p <> [b0]) {
+          while (i < size p - 1 /\ mem (dom m) (sa +^ nth witness p i, sc)) {
+            (sa, sc) <- oget m.[(sa +^ nth witness p i, sc)];
+            (sa', h) <- oget mh.[(sa +^ nth witness p i, h)];
+            i        <- i + 1;
+          }
+          while (i < size p) {
+            sc                  <$ cdistr;
+            sa'                 <- RO.f(take i p);
+            mh.[(sa,h)]         <- (sa', chandle);
+            mhi.[(sa',chandle)] <- (sa,h);
+            (sa,h)              <- (sa',chandle);
+            handles.[chandle]   <- (sc,I);
+            chandle             <- chandle + 1;
+            i                   <- i + 1;
+          }
+          sa <- RO.f(p);
+        }
+        return sa;
+      }
+    }
+
+    module S = {
+      (** Inner interface **)
+      proc f(x : state): state = {
+        var p, v, y, y1, y2, hy2, hx2;
+  
+        if (!mem (dom m) x) {
+          if (mem (dom paths) x.`2) {
+            (p,v) <- oget paths.[x.`2]; 
+            y1    <- RO.f (rcons p (v +^ x.`1));
+            y2    <$ cdistr;
+            y     <- (y1, y2);
+            paths.[y2] <- (rcons p (v +^ x.`1), y.`1);
+          } else {
+            y <$ dstate;
+          }
+          bext <- bext \/ mem (rng handles) (x.`2, I);   
+            (*  exists x2 h, handles.[h] = Some (X2,I) *)
+          if (!(mem (rng handles) (x.`2, D))) {
+            handles.[chandle] <- (x.`2, D);
+            chandle <- chandle + 1;
+          }
+          hx2 <- oget (hinvD handles x.`2);
+          if (mem (dom mh) (x.`1, hx2)) {
+            hy2               <- (oget mh.[(x.`1, hx2)]).`2;
+            handles.[hy2]     <- (y.`2, D);
+            (* bad               <- bad \/ mem X2 y.`2; *)
+            m.[x]             <- y;
+            mh.[(x.`1, hx2)]  <- (y.`1, hy2);
+            mi.[y]            <- x;
+            mhi.[(y.`1, hy2)] <- (x.`1, hx2);
+          } else {
+            hy2               <- chandle;
+            chandle           <- chandle + 1;
+            handles.[hy2]     <- (y.`2, D);
+            m.[x]             <- y;
+            mh.[(x.`1, hx2)]  <- (y.`1, hy2);
+            mi.[y]            <- x;
+            mhi.[(y.`1, hy2)] <- (x.`1, hx2);
+          }
+        } else {   
+          y <- oget m.[x];
+        }
+        return y;
+      }
+
+      proc fi(x : state): state = {
+        var y, y1, y2, hx2, hy2;
+
+        if (!mem (dom mi) x) {
+          bext <- bext \/ mem (rng handles) (x.`2, I);   
+            (*  exists x2 h, handles.[h] = Some (X2,I) *)
+          if (!(mem (rng handles) (x.`2, D))) {
+            handles.[chandle] <- (x.`2, D);
+            chandle <- chandle + 1;
+          }
+          hx2 <- oget (hinvD handles x.`2);
+          if (mem (dom mhi) (x.`1, hx2)) {
+            (y1,hy2)          <- oget mhi.[(x.`1, hx2)];
+            y2                <$ cdistr;
+            y                 <- (y1,y2);
+            handles.[hy2]     <- (y.`2, D);
+            (* bad               <- bad \/ mem X2 y.`2; *)
+            mi.[x]            <- y;
+            mhi.[(x.`1, hx2)] <- (y.`1, hy2);
+            m.[y]             <- x;
+            mh.[(y.`1, hy2)]  <- (x.`1, hx2);
+          } else {
+            y                 <$ dstate;
+            hy2               <- chandle;
+            chandle           <- chandle + 1;
+            handles.[hy2]     <- (y.`2, D);
+            mi.[x]            <- y;
+            mhi.[(x.`1, hx2)] <- (y.`1, hy2);
+            m.[y]             <- x;
+            mh.[(y.`1, hy2)]  <- (x.`1, hx2);
+          }
+        } else {
+          y <- oget mi.[x];
+        }
+        return y;
+      }
+
+      (** Distinguisher interface **)
+      proc init() = { }
+
+    }
+
+  
+
+    proc main(): bool = {
+      var b;
+
+      m        <- map0;
+      mi       <- map0;
+      bext     <- false;
+
+      (* the empty path is initially known by the adversary to lead to capacity 0^c *)
+      handles  <- map0.[0 <- (c0, D)];
+      paths    <- map0.[c0 <- ([<:block>],b0)];
+      chandle  <- 1;
+      b        <@ D(C,S).distinguish();
+      return b;
+    }    
+  }.
+
+
+
+
+  local module Game1 = {
+    var m, mi               : (hstate,hstate) fmap
+    var paths               : (handle,(block list * block) list) fmap
+    var handles             : (handle, ccapacity) fmap
+    var bext, bred, bcoll   : bool
+    var chandle             : int
 
     module S = {
       (** Inner interface **)
       proc fg(o : caller, x : state): state = {
-        var o', y, pv, p, v;
+        var o', p, v, y, y1, y2, ox2, hx2, y1h;
+  
+        ox2  <- hinv handles x.`2;
+        hx2  <- oget ox2;
+        bext <- bext \/ 
+                (o = D /\ ox2 <> None  /\ paths.[hx2] <> None /\ 
+                find_path m D paths hx2 = None);
 
-        o' <- odflt D pathscol.[x.`2];
-        bext <- bext \/ (o' <= o);
 
-        if (!mem (dom m) x) {
-          y <$ dstate;
-          if (mem (dom paths) x.`2) {
-            o'              <- oget pathscol.[x.`2];
-            pv              <- oget paths.[x.`2];
-            (p,v)           <- pv;
-            bcoll           <- bcoll \/ (mem (dom paths) y.`2);
-            bsuff           <- bsuff \/ (mem (image snd (rng m)) y.`2);
-            pathscol.[y.`2] <- max o o';
-            paths.[y.`2]    <- (rcons p (v ^ x.`1),y.`1);
-          }
-          mcol.[x]  <- o;
-          m.[x]     <- y;
-          micol.[y] <- o;
-          mi.[y]    <- x;
-        } else {
-          o'        <- oget mcol.[x];
-          mcol.[x]  <- max o o';
-          y         <- oget m.[x];
-          o'        <- oget micol.[y];
-          micol.[y] <- max o o';
+        if (ox2 = None) {
+           handles.[chandle] <- (x.`2,o);
+           hx2               <- chandle;
+           chandle           <- chandle + 1;
         }
-        return oget m.[x];
+        
+        if (!mem (dom m) (x.`1, hx2) || (oget handles.[hx2]).`2 = I /\ o = D) { 
+          if (mem (dom paths) hx2 /\ find_path m o paths hx2 <> None) {
+            (p,v) <- oget (find_path m o paths hx2);
+            y1    <- RO.f (rcons p (v +^ x.`1));
+            y2    <$ cdistr;
+            y     <- (y1, y2);
+            if (hinv handles y.`2 = None) 
+              paths.[chandle (*y2*)] <- extend_paths x.`1 y.`1 (oget paths.[hx2]);
+          } else {
+            y <$ dstate;
+          }
+          if (hinv handles y.`2 = None) {
+            y1h               <- (y.`1, chandle);
+            handles.[chandle] <- (y.`2, o);
+            m.[(x.`1, hx2)]   <- y1h;
+            mi.[y1h]          <- (x.`1, hx2);
+            handles.[hx2]     <- (x.`2, max o (oget handles.[hx2]).`2);   (* Warning: not sure we want it *)
+            chandle           <- chandle + 1;
+          } else {
+            bcoll <- true;
+          }
+        } else {   (* mem (dom m) (x.`1, hx2) /\ (!dom m with I \/ o <> D) *)  
+          y1h              <- oget m.[(x.`1,hx2)];
+          (y2,o')          <- oget handles.[y1h.`2];   
+          handles.[y1h.`2] <- (y2, max o o');  
+          handles.[hx2]    <- (x.`2, max o (oget handles.[hx2]).`2);
+          y                <- (y1h.`1, y2);
+        }
+        return y;
       }
 
       proc f(x:state):state = {
@@ -411,23 +729,40 @@ print FUNCTIONALITY.
       }
 
       proc fi(x : state): state = {
-        var o', y;
+        var o', y, y2, ox2, hx2, y1h;
 
-        if (!mem (dom mi) x) {
-          y <$ dstate;
-          micol.[x] <- D;
-          mi.[x]    <- y;
-          mcol.[y]  <- D;
-          m.[y]     <- x;
-          bmitm     <- bmitm \/ (mem (dom paths) y.`2);
-        } else {
-          o'        <- oget micol.[x];
-          bred      <- bred \/ o' = I;
-          y         <- oget mi.[x];
-          micol.[x] <- D;
-          mcol.[y]  <- D;
+        ox2  <- hinv handles x.`2;
+        hx2  <- oget ox2;
+
+        if (ox2 = None) {
+           handles.[chandle] <- (x.`2,D);
+           hx2               <- chandle;
+           chandle           <- chandle + 1;
         }
-        return oget mi.[x];
+        
+        if (!mem (dom mi) (x.`1,hx2) || (oget handles.[hx2]).`2 = I) {
+          y                 <$ dstate;
+          if ( hinv handles y.`2 = None) {
+            y1h               <- (y.`1, chandle);
+            handles.[chandle] <- (y.`2, D);
+            mi.[(x.`1, hx2)]  <- y1h; 
+            m.[y1h]           <- (x.`1, hx2);
+            handles.[hx2]     <- ((oget handles.[hx2]).`1, D);
+            chandle           <- chandle + 1;     
+          } else {
+            bcoll <- true;
+          }
+
+        } else {
+          y1h              <- oget mi.[(x.`1,hx2)];
+          (y2,o')          <- oget handles.[y1h.`2];   
+          bred             <- bred \/ o' = I; 
+          handles.[y1h.`2] <- (y2, D);  
+          handles.[hx2]    <- (x.`2, D);
+          y                <- (y1h.`1, y2);
+
+        }
+        return y;
       }
 
       (** Distinguisher interface **)
@@ -439,9 +774,9 @@ print FUNCTIONALITY.
       proc init(): unit = { }
 
       proc f(p : block list): block = {
-        var (sa,sc) <- (Block.zeros,Capacity.zeros);
+        var (sa,sc) <- (b0,c0);
 
-        if (1 <= size p /\ p <> [Block.zeros]) {
+        if (1 <= size p /\ p <> [b0]) {
           while (p <> []) {
             (sa,sc) <@ S.fg(I,(sa ^ head witness p,sc));
             p <- behead p;
@@ -454,9 +789,7 @@ print FUNCTIONALITY.
     proc main(): bool = {
       var b;
 
-      mcol     <- map0;
       m        <- map0;
-      micol    <- map0;
       mi       <- map0;
       bext     <- false;
       bred     <- false;
@@ -464,12 +797,87 @@ print FUNCTIONALITY.
       bsuff    <- false;
       bmitm    <- false;
       (* the empty path is initially known by the adversary to lead to capacity 0^c *)
-      pathscol <- map0.[Capacity.zeros <- D];
-      paths    <- map0.[Capacity.zeros <- ([<:block>],Block.zeros)];
+      handles  <- map0.[0 <- (c0, D)];
+      paths    <- map0.[0 <- ([<:block>],b0,D)];
+      chandle  <- 1;
       b        <@ D(C,S).distinguish();
       return b;
     }    
   }.
+
+
+
+
+
+module M = {
+   proc f () : unit = {
+      var x;
+      var l:int list;
+      l = [];
+  }
+}.
+
+
+
+
+
+
+
+
+
+
+
+
+
+
+
+
+
+
+
+
+
+
+
+
+
+
+
+
+
+
+
+
+
+
+
+
+
+
+
+
+
+
+
+
+
+
+
+
+
+
+
+
+
+
+
+
+
+
+
+
+
+
 
   (** Result: the instrumented system and the concrete system are
       perfectly equivalent **)
@@ -619,9 +1027,9 @@ print FUNCTIONALITY.
       proc init(): unit = { }
 
       proc f(p : block list): block = {
-        var (sa,sc) <- (Block.zeros,Capacity.zeros);
+        var (sa,sc) <- (b0,c0);
 
-        if (1<= size p /\ p <> [Block.zeros]) {
+        if (1<= size p /\ p <> [b0]) {
           while (p <> []) {
             (sa,sc) <@ S.fg(I,(sa ^ head witness p,sc));
             p <- behead p;
@@ -646,8 +1054,8 @@ print FUNCTIONALITY.
       bsuff    <- false;
       bmitm    <- false;
       (* the empty path is initially known by the adversary to lead to capacity 0^c *)
-      pathscol <- map0.[Capacity.zeros <- D];
-      paths    <- map0.[Capacity.zeros <- ([<:block>],Block.zeros)];
+      pathscol <- map0.[c0 <- D];
+      paths    <- map0.[c0 <- ([<:block>],b0)];
       b        <@ D(C,S).distinguish();
       return b;
     }    
@@ -721,6 +1129,133 @@ print FUNCTIONALITY.
       by wp; call Game1_S_S_eq.
     by auto; smt.
   qed.
+
+(*un jeu avec indirection.
+jeu avec indirection -> simulateur. *)
+  type handle = int.
+  type hstate = block * handle.
+
+
+  local module Game2 = {
+    
+    var mcol,micol          : (hstate,caller) fmap
+    var rate, ratei         : (hstate,block) fmap
+    var cap, capi           : (hstate,handle) fmap
+    var handles             : (handle,capacity) fmap                
+    var pathscol            : (handle,caller) fmap
+    var paths               : (handle,block list * block) fmap
+    var bext, bred          : bool
+    var bcoll, bsuff, bmitm : bool
+
+    module S = {
+      (** Inner interface **)
+      proc fg(o : caller, x : state): state = {
+        var o', ya, yc, pv, p, v, x2;
+   
+        (* Fait chier ici *)
+(*        o' <- odflt D pathscol.[x.`2];
+          bext <- bext \/ (o' <= o); *)
+
+        if (!mem (dom rate) x) {
+          x2 <- hinv handles x.`2;        
+          (ya,yc) <$ dstate;
+          if (mem (dom paths) x.`2) {
+            o'            <- oget pathscol.[x.`2];
+            pv            <- oget paths.[x.`2];
+            (p,v)         <- pv;
+            bcoll         <- bcoll \/ (mem (dom paths) yc);
+            bsuff         <- bsuff \/ (mem (rng cap) yc);
+            pathscol.[yc] <- max o o';
+            paths.[yc]    <- (rcons p (v ^ x.`1),ya);
+          }
+          rate.[x]        <- ya;
+          ratei.[(ya,yc)] <- x.`1;
+          cap.[x]         <- yc;
+          capi.[(ya,yc)]  <- x.`2;
+          mcol.[x]        <- o;
+          micol.[(ya,yc)] <- o;
+        } else {
+          o'              <- oget mcol.[x];
+          mcol.[x]        <- max o o';
+          ya              <- oget rate.[x];
+          yc              <- oget cap.[x];
+          o'              <- oget micol.[(ya,yc)];
+          micol.[(ya,yc)] <- max o o';
+        }
+        return (oget rate.[x],oget cap.[x]);
+      }
+
+      proc f(x:state):state = {
+        var r; 
+        r <@ fg(D,x);
+        return r;
+      }
+
+      proc fi(x : state): state = {
+        var ya, yc;
+
+        if (!mem (dom ratei) x) {
+          (ya,yc)        <$ dstate;
+          micol.[x]      <- D;
+          ratei.[x]      <- ya;
+          capi.[x]       <- yc;
+          mcol.[(ya,yc)] <- D;
+          rate.[(ya,yc)] <- x.`1;
+          cap.[(ya,yc)]  <- x.`2;
+          bmitm  <- bmitm \/ (mem (dom paths) yc);
+        } else {
+          bred           <- bred \/ oget micol.[x] = I;
+          micol.[x]      <- D;
+          ya             <- oget ratei.[x];
+          yc             <- oget capi.[x];
+          mcol.[(ya,yc)] <- D;
+        }
+        return (oget ratei.[x],oget capi.[x]);
+      }
+
+      (** Distinguisher interface **)
+      proc init() = { }
+
+    }
+
+    module C = {
+      proc init(): unit = { }
+
+      proc f(p : block list): block = {
+        var (sa,sc) <- (b0,c0);
+
+        if (1<= size p /\ p <> [b0]) {
+          while (p <> []) {
+            (sa,sc) <@ S.fg(I,(sa ^ head witness p,sc));
+            p <- behead p;
+          }
+        }
+        return sa;
+      }
+    }
+
+    proc main(): bool = {
+      var b;
+
+      mcol     <- map0;
+      micol    <- map0;
+      rate     <- map0;
+      ratei    <- map0;
+      cap      <- map0;
+      capi     <- map0;
+      bext     <- false;
+      bred     <- false;
+      bcoll    <- false;
+      bsuff    <- false;
+      bmitm    <- false;
+      (* the empty path is initially known by the adversary to lead to capacity 0^c *)
+      pathscol <- map0.[c0 <- D];
+      paths    <- map0.[c0 <- ([<:block>],b0)];
+      b        <@ D(C,S).distinguish();
+      return b;
+    }    
+  }.
+
 end section.
 
 (* That Self is unfortunate *)
